running the mul exception example inside Coq works

src/riscv/Examples/MulTrapHandler.v
@@ -28,7 +28,7 @@ Require Import riscv.Platform.LogInstructionTrace.
 (* note: these numbers must fit into a 12bit immediate, and should be small if we want to simulate
    execution inside Coq *)
 Definition main_start: Z := 0.
-Definition handler_start: Z := 16.
+Definition handler_start: Z := 32.
 Definition handler_stack_start: Z := 512.
 Definition heap_start: Z := 640.
 
@@ -43,15 +43,16 @@ Definition main_insts := [[
 (* a3 := a1 * a2
    without using mul, but with a naive loop:
    a3 := 0;
-   while (0 < a1) {
+   while (0 != a1) {
      a3 := a3 + a2;
      a1 := a1 - 1;
    } *)
 Definition softmul_insts := [[
   Addi a3 zero 0;
-  Bltu zero a1 8;
+  Beq zero a1 16;
   Add a3 a3 a2;
-  Addi a1 a1 (-1)
+  Addi a1 a1 (-1);
+  J (-12)
 ]].
 
 (* We also save the constant register 0 on the stack, so that we can conveniently index into an
@@ -66,38 +67,43 @@ Definition restore_regs_insts(addr: Z) :=
 (* TODO write encoder (so far there's only a decoder called CSR.lookupCSR) *)
 Definition MTVal: MachineInt := 835.
 Remark MTVal_correct: CSR.lookupCSR MTVal = CSR.MTVal. reflexivity. Qed.
+Definition MEPC: MachineInt := 833.
+Remark MEPC_correct: CSR.lookupCSR MEPC = CSR.MEPC. reflexivity. Qed.
 
 Definition handler_insts :=
   save_regs_insts handler_stack_start ++ [[
   Csrr t1 MTVal                    ; (* t1 := the invalid instruction i that caused the exception *)
-  Srli t1 t1 7                     ; (* t1 := t1 >> 7                                             *)
-  Andi s3 t1 31                    ; (* s3 := i[7:12]   // rd of the MUL                          *)
-  Srli t1 t1 3                     ; (* t1 := t1 >> 3                                             *)
-  Andi s1 t1 31                    ; (* s1 := i[15:20]  // rs1 of the MUL                         *)
   Srli t1 t1 5                     ; (* t1 := t1 >> 5                                             *)
-  Andi s2 t1 31                    ; (* s2 := i[20:25]  // rs2 of the MUL                         *)
+  Andi s3 t1 (31*4)                ; (* s3 := i[7:12]<<2   // (rd of the MUL)*4                   *)
+  Srli t1 t1 8                     ; (* t1 := t1 >> 8                                             *)
+  Andi s1 t1 (31*4)                ; (* s1 := i[15:20]<<2  // (rs1 of the MUL)*4                  *)
+  Srli t1 t1 5                     ; (* t1 := t1 >> 5                                             *)
+  Andi s2 t1 (31*4)                ; (* s2 := i[20:25]<<2  // (rs2 of the MUL)*4                  *)
   Lw a1 s1 handler_stack_start     ; (* a1 := stack[s1]                                           *)
   Lw a2 s2 handler_stack_start       (* a2 := stack[s2]                                           *)
   ]] ++ softmul_insts ++ [[          (* a3 := softmul(a1, a2)                                     *)
   Sw s3 a3 handler_stack_start       (* stack[s3] := a3                                           *)
   ]] ++ restore_regs_insts handler_stack_start ++ [[
+  Csrr t1 MEPC                     ;
+  Addi t1 t1 4                     ;
+  Csrw t1 MEPC                     ; (* MEPC := MEPC + 4                                          *)
   Mret
   ]].
 
-Definition all_insts := main_insts ++ handler_insts.
-
-Definition insts_as_Zs: list Z := Eval vm_compute in List.map encode all_insts.
-
-Definition program_size := Eval vm_compute in 4 * Z.of_nat (length insts_as_Zs).
+Definition input1: Z := 5.
+Definition input2: Z := 13.
 
 Definition initial_datamem: Mem := Eval vm_compute in
-      map.put (map.put (map.of_tuple (Memory.footprint (word.of_Z handler_stack_start) 300)
-                            (HList.tuple.unfoldn id 300 Byte.x00))
-                       (word.of_Z heap_start) Byte.x03)
-              (word.of_Z (heap_start+4)) Byte.x04.
+      let m := map.of_tuple (Memory.footprint (word.of_Z handler_stack_start) 300)
+                            (HList.tuple.unfoldn id 300 Byte.x00) in
+      let m := unchecked_store_bytes 4 m (word.of_Z heap_start) (LittleEndian.split 4 input1) in
+      unchecked_store_bytes 4 m (word.of_Z (heap_start+4)) (LittleEndian.split 4 input2).
+
+Definition putProgram(m: Mem)(addr: Z)(prog: list Instruction): Mem :=
+  unchecked_store_byte_list (word.of_Z addr) (RiscvMachine.Z32s_to_bytes (List.map encode prog)) m.
 
 Definition initial_mem: Mem := Eval vm_compute in
-  unchecked_store_byte_list (word.of_Z 0) (RiscvMachine.Z32s_to_bytes insts_as_Zs) initial_datamem.
+  putProgram (putProgram initial_datamem main_start main_insts) handler_start handler_insts.
 
 Definition FieldNames: natmap Type := MinimalCSRsDet.Fields (natmap.put nil exectrace ExecTrace).
 
@@ -135,5 +141,16 @@ Definition trace(fuel: nat): bool * ExecTrace :=
   | (isSuccess, final) => (isSuccess, final[exectrace])
   end.
 
-Eval vm_compute in trace 83.
-(* oh no, Mret jumps back to the Mul that caused the exception instead of one past the Mul *)
+(* fails, but that's excpected because it runs past the last instruction of main into unmapped memory
+Eval vm_compute in trace 1000. *)
+
+Goal Memory.loadWord initial_state[mem] (word.of_Z (heap_start+8)) = Some (LittleEndian.split 4 0).
+Proof. reflexivity. Qed.
+
+Goal Memory.loadWord initial_state[mem] (word.of_Z (heap_start+8)) =
+     Some (LittleEndian.split 4 0).
+Proof. reflexivity. Qed.
+
+Goal Memory.loadWord (snd (run 1000 initial_state))[mem] (word.of_Z (heap_start+8)) =
+     Some (LittleEndian.split 4 (input1 * input2)).
+Proof. vm_compute. reflexivity. Qed.
